basic_fallible_transform.thy
@@ -50,6 +50,11 @@ lemma ftransform_has_result[NER_simps]:
   "has_result (ftransform_p t p) i r l \<longleftrightarrow> (\<exists> r'. has_result p i r' l \<and> t r' = Some r)"
   by (auto simp add: ftransform_def has_result_def split: option.splits)
 
+lemma ftransform_has_result_c[NER_simps]:
+  "has_result_c (parse (ftransform t t' bi)) c r l \<longleftrightarrow> (\<exists> r'. has_result_c (parse bi) c r' l \<and> t r' = Some r)"
+  "has_result_c (ftransform_p t p)           c r l \<longleftrightarrow> (\<exists> r'. has_result_c p c r' l \<and> t r' = Some r)"
+  by (auto simp add: ftransform_def has_result_c_def NER_simps split: option.splits)
+
 
 
 \<comment> \<open>FP NER\<close>
